% SPDX-FileCopyrightText: Copyright (C) Nile Jocson <novoseiversia@gmail.com>
% SPDX-License-Identifier: MPL-2.0

\documentclass{article}

\input{../../common/cjmath.tex}



\begin{document}
	\cjboilerplate{Math 20}{Linear, Quadratic, and Rational Equations}

	\begin{cjsection}{}
		\cjitem{Find the solution set of the following equations.}
			\cjsubitem{\(x + 9 = 5 - 3x\)}
				\begin{cjsolution}
					\cjwhy{\(x + 3x = 5 - 9\)}{Solve for \(x\).}
					\cjcontinue{\(4x = -4\)}
					\cjcontinue{\(x = -1\)}
				\end{cjsolution}

			\cjsubitem{\(\frac{2x + 3}{4} - \frac{x - 1}{2} = -\frac{1}{3}\)}
				\begin{cjsolution}
					\cjwhy{\(\frac{3(2x + 3)}{12} - \frac{6(x - 1)}{12} = -\frac{4}{12}\)}{\(\text{LCM} = 12\)}
					\cjcontinue{\(\frac{6x + 9}{12} - \frac{6x - 6}{12} = -\frac{4}{12}\)}
					\cjcontinue{\((6x + 9) - (6x - 6) = -4\)}
					\cjcontinue{\(6x + 9 - 6x + 6 = -4\)}
					\cjcontinue{\(15 = -4\)}
					\cjcontinue{\(x = \emptyset\)}
				\end{cjsolution}

			\cjsubitem{\(3x^2 - 2x + 1 = 0\)}
				\begin{cjsolution}
					\cjwhy{\(\frac{-(-2) \pm \sqrt{{(-2)}^2 - 4(3)(1)}}{2(3)}\)}{Use the quadratic formula.}
					\cjcontinue{\(\frac{2 \pm \sqrt{-8}}{6}\)}
					\cjcontinue{\(\frac{2 \pm \sqrt{4}\sqrt{-2}}{6}\)}
					\cjcontinue{\(\frac{2 \pm 2i\sqrt{2}}{6}\)}
					\cjcontinue{\(\frac{1 \pm i\sqrt{2}}{3}\)}
					\cjcontinue{\(\frac{1}{3} \pm \frac{\sqrt{2}}{3}i\)}
					\cjcontinue{\(x = \{\frac{1}{3} + \frac{\sqrt{2}}{3}i, \frac{1}{3} - \frac{\sqrt{2}}{3}i\}\)}
				\end{cjsolution}

			\cjsubitem{\(4x^2 + 2x = 2\)}
				\begin{cjsolution}
					\cjwhy{\(4x^2 + 2x - 2 = 0\)}{Rewrite in standard form.}
					\cjcontinue{\(2x^2 + x - 1 = 0\)}
					\cjwhy{\(2x^2 + 2x - x - 1 = 0\)}{Factor by grouping.}
					\cjcontinue{\(2x(x + 1) - 1(x + 1) = 0\)}
					\cjcontinue{\((2x - 1)(x + 1) = 0\)}
					\cjcontinue{\(x = \{-1, \frac{1}{2}\}\)}
				\end{cjsolution}

			\cjsubitem{\(16x^2 + 9 = 24x\)}
				\begin{cjsolution}
					\cjwhy{\(16x^2 - 24x + 9 = 0\)}{Rewrite in standard form.}
					\cjwhy{\(16x^2 - 12x - 12x + 9 = 0\)}{Factor by grouping.}
					\cjcontinue{\(4x(4x - 3) - 3(4x - 3) = 0\)}
					\cjcontinue{\({(4x - 3)}^2 = 0\)}
					\cjcontinue{\(x = \frac{3}{4}\)}
				\end{cjsolution}

			\cjsubitem{\(\frac{x}{x - 1} + \frac{x - 5}{x^2 + 2x - 3} = \frac{1}{x + 3}\)}
				\begin{cjsolution}
					\cjwhy{\(\frac{x}{x - 1} + \frac{x - 5}{(x - 1)(x + 3)} = \frac{1}{x + 3}\)}{Factor by grouping.}
					\cjwhy{\(\frac{x(x + 3)}{(x - 1)(x + 3)} + \frac{x - 5}{(x - 1)(x + 3)} = \frac{x - 1}{(x - 1)(x + 3)}\)}{\(\text{LCM} = (x - 1)(x + 3)\)}
					\cjcontinue{\(\frac{x^2 + 3x}{(x - 1)(x + 3)} + \frac{x - 5}{(x - 1)(x + 3)} = \frac{x - 1}{(x - 1)(x + 3)}\)}
					\cjwhy{\(x^2 + 3x + x - 5 = x - 1\)}{Eliminate denominator. \(x \in \{-3, 1\}\) are undefined points.}
					\cjcontinue{\(x^2 + 3x + x - 5 - x + 1 = 0\)}
					\cjcontinue{\(x^2 + 3x - 4 = 0\)}
					\cjwhy{\((x + 4)(x - 1) = 0\)}{Factor by grouping.}
					\cjcontinue{\(x = -4\)}
				\end{cjsolution}
	\end{cjsection}
\end{document}
